lakefile.lean
@@ -1,11 +1,7 @@
 import Lake
 open Lake DSL
 
-package «STLC» {
-  -- add package configuration options here
-}
+package STLC
 
 @[default_target]
-lean_lib «STLC» {
-  -- add library configuration options here
-}
+lean_lib STLC
